Cook_Levin/IMP-_To_SAS+/IMP_Minus_To_SAT_Nat.thy
@@ -1,5 +1,6 @@
 theory IMP_Minus_To_SAT_Nat 
-  imports IMP_Minus_To_SAS_Plus_Nat IMP_Minus_To_SAT SAT_Plan_Base_Nat "IMP-_To_IMP--/Primitives"  
+  imports IMP_Minus_To_SAS_Plus_Nat IMP_Minus_To_SAT SAT_Plan_Base_Nat SAS_Plus_Strips_Nat
+ "IMP-_To_IMP--/Primitives"  
 begin
 
 fun poly_of :: "nat*nat \<Rightarrow> nat \<Rightarrow> nat" where 
@@ -90,6 +91,20 @@ lemma sublist_prob_with_noop:
   apply (auto simp add: prob_with_noop_list_def prob_with_noop_def)
   done
 
+definition prob_with_noop_nat :: "nat \<Rightarrow> nat" where 
+  "prob_with_noop_nat p = (nth_nat 0 p) ## ( empty_sasp_action_nat ##  (nth_nat (Suc 0) p))
+## (tl_nat (tl_nat p))"
+
+lemma subnat_prob_with_noop: 
+"prob_with_noop_nat (list_problem_plus_encode p) = 
+ list_problem_plus_encode (prob_with_noop_list p)"
+  apply (auto simp only: prob_with_noop_nat_def sub_cons list_problem_plus_encode_def
+            sub_tl tail.simps sub_nth nth.simps prob_with_noop_list_def sas_plus_list_problem.simps
+            sub_empty_sasp_action)
+  apply auto
+  done
+
+
 definition encode_interfering_operator_pair_exclusion_list
   :: "'variable strips_list_problem
     \<Rightarrow> nat
@@ -109,6 +124,75 @@ lemma sublist_encode_interfering_operator_pair_exclusion:
 encode_interfering_operator_pair_exclusion_def)
   done
 
+definition encode_interfering_operator_pair_exclusion_nat
+  :: "nat
+    \<Rightarrow> nat
+    \<Rightarrow> nat
+    \<Rightarrow> nat
+    \<Rightarrow> nat"
+  where "encode_interfering_operator_pair_exclusion_nat p k o1 o2
+    \<equiv> let ops = nth_nat (Suc 0)  p in
+     4 ## (2 ## (1 ## (1 ## k ## (index_nat ops o1)## 0) ## 0) ## 0)
+      ## (2 ## (1 ## (1  ## k ## (index_nat ops o2) ## 0) ## 0) ## 0) ## 0"
+
+lemma subnat_encode_interfering_operator_pair_exclusion:
+"encode_interfering_operator_pair_exclusion_nat (strips_list_problem_encode p) k
+ (strips_operator_encode o1) (strips_operator_encode o2) = 
+sat_formula_encode (encode_interfering_operator_pair_exclusion_list p k o1 o2)"
+  using inj_strips_op
+  apply(auto simp only: encode_interfering_operator_pair_exclusion_nat_def
+    strips_list_problem_encode.simps sub_nth nth.simps strips_operator_list_encode_def
+      sub_index Let_def sub_cons cons0 encode_interfering_operator_pair_exclusion_list_def
+ simp flip: sat_variable_encode.simps sat_formula_encode.simps
+)
+  done
+
+
+declare elemof.simps [simp del]
+fun list_inter :: "nat \<Rightarrow> nat \<Rightarrow> nat" where 
+"list_inter xs ys = (if xs = 0 then 0 
+else if elemof (hd_nat xs) ys \<noteq> 0 then 1 else list_inter (tl_nat xs) ys)"
+
+lemma list_encode_pos:"(list_encode xs > 0) = (xs \<noteq> []) "
+  using list_encode_empty by force
+
+lemma sub_list_inter:
+"inj f \<Longrightarrow> list_inter (list_encode (map f xs)) (list_encode (map f ys)) \<noteq> 0 
+= list_ex (\<lambda>v. list_ex ((=) v) xs ) ys"
+  apply (induct xs)
+   apply (simp)
+   apply (induct ys)
+    apply simp
+   apply simp
+  apply (subst list_inter.simps)
+  apply (simp add: sub_hd sub_tl tail.simps  head.simps list.simps list_encode_empty list_encode_pos
+      del:list_encode.simps list_inter.simps)
+  using sub_elem_of_inj[of f] apply (auto simp  del:list_encode.simps list_inter.simps)
+  apply (metis (no_types, lifting) Bex_set) 
+    apply (metis (no_types, lifting) Bex_set)
+  using Bex_set apply fastforce
+ using sub_elem_of_inj[of f]
+  by (smt (z3) Bex_set)
+    
+
+
+
+definition are_operators_interfering_nat :: "nat \<Rightarrow> nat \<Rightarrow> nat" where
+"are_operators_interfering_nat o1 o2 \<equiv>
+if list_inter (nth_nat (Suc (Suc 0)) o1) (nth_nat 0 o2) \<noteq> 0  \<or> 
+    list_inter (nth_nat 0 o1) (nth_nat (Suc (Suc 0)) o2) \<noteq> 0 then 1 else 0 "
+
+lemma sub_are_operators_interfering:
+"(are_operators_interfering_nat (strips_operator_encode o1) (strips_operator_encode o2) > 0) =
+ (are_operators_interfering o1 o2)"
+  using inj_sasp
+  apply (auto simp only: are_operators_interfering_nat_def strips_operator_encode.simps
+          sub_nth nth.simps sas_plus_assignment_list_encode_def
+            sub_list_inter are_operators_interfering_def)
+    apply auto
+  apply presburger
+  done
+  
 
 definition encode_interfering_operator_exclusion_list
   :: "'variable strips_list_problem \<Rightarrow> nat \<Rightarrow> sat_plan_variable formula"
@@ -128,6 +212,42 @@ encode_interfering_operator_exclusion_def
 )
   done
 
+definition encode_interfering_operator_exclusion_nat
+  :: "nat \<Rightarrow> nat \<Rightarrow> nat"
+  where "encode_interfering_operator_exclusion_nat \<Pi> t \<equiv> let
+      ops = nth_nat (Suc 0) \<Pi>
+      ; interfering = filter_nat (\<lambda>n. index_nat ops (fst_nat n) \<noteq> index_nat ops (snd_nat n)
+        \<and> are_operators_interfering_nat (fst_nat n) (snd_nat n) \<noteq> 0 ) (product_nat ops ops)
+    in BigAnd_nat (concat_nat (map_nat (\<lambda>n. map_nat (\<lambda>k. encode_interfering_operator_pair_exclusion_nat \<Pi> k (fst_nat n) (snd_nat n))
+      (list_less_nat t) ) interfering ))"
+lemma subnat_encode_interfering_operator_exclusion :
+"encode_interfering_operator_exclusion_nat (strips_list_problem_encode p) t =
+sat_formula_encode (encode_interfering_operator_exclusion_list p t)"
+  using inj_strips_op
+  apply (auto simp only: encode_interfering_operator_exclusion_nat_def 
+strips_list_problem_encode.simps sub_nth nth.simps Let_def strips_operator_list_encode_def
+sub_product sub_filter filter_map
+         )
+  apply (auto simp add: Fun.comp_def prod.case_eq_if sub_fst sub_snd simp del: list_encode.simps 
+          BigAnd_nat.simps concat_nat.simps index_nat.simps strips_operator_encode.simps
+        map_nat.simps simp flip: strips_operator_list_encode_def  strips_list_problem_encode.simps)
+  apply (auto simp only:  strips_operator_list_encode_def sub_index sub_are_operators_interfering
+      sub_map map_map Fun.comp_def  prod.case_eq_if  sub_fst sub_snd fst_conv snd_conv sub_list_less
+            subnat_encode_interfering_operator_pair_exclusion
+            )
+  apply (auto simp only: sub_concat  simp flip: Fun.comp_def[of list_encode "\<lambda>x. 
+    (map (\<lambda>k. sat_formula_encode
+                (encode_interfering_operator_pair_exclusion_list p k (fst x) (snd x)))
+                       [0..<t])" ] map_map map_concat)
+  apply (auto simp only: simp flip: Fun.comp_def[of sat_formula_encode 
+            "\<lambda>k. encode_interfering_operator_pair_exclusion_list p k (fst _) (snd _)"] map_map
+)
+  apply (auto simp only: case_prod_beta' sub_BigAnd encode_interfering_operator_exclusion_list_def split_comp_eq 
+      Let_def simp flip: Fun.comp_def[of "map sat_formula_encode"
+"\<lambda>x. (map (\<lambda>k. encode_interfering_operator_pair_exclusion_list p k (fst x) (snd x))
+                       [0..<t])"] map_map map_concat sat_formula_list_encode_def split_comp_eq)
+  done
+
 definition encode_problem_with_operator_interference_exclusion_list
   :: "'variable strips_list_problem \<Rightarrow> nat \<Rightarrow> sat_plan_variable formula"
   where "encode_problem_with_operator_interference_exclusion_list \<Pi> t
@@ -136,6 +256,25 @@ definition encode_problem_with_operator_interference_exclusion_list
       \<^bold>\<and> (encode_all_frame_axioms_list \<Pi> t
       \<^bold>\<and> (encode_interfering_operator_exclusion_list \<Pi> t
       \<^bold>\<and> (encode_goal_state_list \<Pi> t))))"
+
+definition encode_problem_with_operator_interference_exclusion_nat
+  :: "nat\<Rightarrow> nat \<Rightarrow> nat"
+  where "encode_problem_with_operator_interference_exclusion_nat \<Pi> t
+    \<equiv> 3 ## (encode_initial_state_nat \<Pi>)
+      ## (3 ## (encode_operators_nat \<Pi> t)
+      ## (3 ## (encode_all_frame_axioms_nat \<Pi> t)
+      ## (3 ## (encode_interfering_operator_exclusion_nat \<Pi> t)
+      ## (encode_goal_state_nat \<Pi> t) ## 0) ## 0 )## 0) ## 0"
+
+lemma subnat_encode_problem_with_operator_interference_exclusion:
+"encode_problem_with_operator_interference_exclusion_nat (strips_list_problem_encode \<Pi>) t =
+sat_formula_encode (encode_problem_with_operator_interference_exclusion_list \<Pi> t)"
+  apply (auto simp only:encode_problem_with_operator_interference_exclusion_nat_def
+    sub_cons cons0 subnat_encode_initial_state subnat_encode_operators subnat_encode_all_frame_axioms
+subnat_encode_interfering_operator_exclusion subnat_encode_goal_state simp flip: sat_formula_encode.simps
+    encode_problem_with_operator_interference_exclusion_list_def
+)
+  done
 
 lemma sublist_encode_problem_with_operator_interference_exclusion:
 "encode_problem_with_operator_interference_exclusion_list \<Pi> t
@@ -153,10 +292,156 @@ encode_problem_with_operator_interference_exclusion_def
       (let I = [(''input'', x)]; 
           G = [(''input'',0)];
           guess_range = x + 1 + 2 * 2 ^ (poly_of p_cer (bit_length x));
-          max_bits = max_input_bits c I guess_range
+          max_bits = max_input_bits_list c I guess_range
       in
-        \<Phi>\<^sub>\<forall> (\<phi> prob_with_noop (IMP_Minus_to_SAS_Plus c I guess_range G (t'_pair pt p_cer x)))
-           100 * (max_bits + (t'_pair pt p_cer x) + 1) * ((t'_pair pt p_cer x) - 1) +
-             (max_bits + (t'_pair pt p_cer x) + 2) * (num_variables c + 2) + 52)"
+        encode_problem_with_operator_interference_exclusion_list 
+        (sas_plus_problem_to_strips_problem_list (prob_with_noop_list (IMP_Minus_to_SAS_Plus_list c I guess_range G (t'_pair pt p_cer x))))
+           (100 * (max_bits + (t'_pair pt p_cer x) + 1) * ((t'_pair pt p_cer x) - 1) +
+             (max_bits + (t'_pair pt p_cer x) + 2) * (num_variables c + 2) + 52))"
+
+lemma sublist_imp_to_sat:
+"imp_to_sat_list c pt p_cer x 
+= imp_to_sat c (poly_of pt) (poly_of p_cer) x"
+  apply (auto simp only: imp_to_sat_list_def sublist_encode_problem_with_operator_interference_exclusion
+              sublist_sas_plus_problem_to_strips_problem sublist_prob_with_noop  sublist_max_input_bits
+                  subpair_t' imp_to_sat_def Let_def)
+  using sublist_IMP_Minus_to_SAS_Plus[of " [(''input'', x)]"] sublist_max_input_bits[of " [(''input'', x)]"]
+  apply (auto)
+  done
+
+lemma poly_poly_of:"poly (poly_of p)"
+  apply(cases p)
+  subgoal for a b
+  proof (induct b arbitrary:p)
+    case 0
+    then have "poly_of p = (\<lambda>_.a)" using poly_of.simps(1) by presburger
+    then show ?case by auto
+  next
+    case (Suc b)
+    then obtain p' where p'_def: "p' = poly_of (a,b)" by blast
+    then have "poly p'" using Suc by simp
+    moreover have "poly_of p = (\<lambda>x. (p' x *x))" using Suc p'_def by force
+    ultimately show ?case apply auto
+      using poly_linear poly_mult by presburger
+  qed
+  done
+
+lemma main_lemma_hol_list:
+  fixes c pt p_cer in_lang
+  assumes verifier_tbounded:
+  (*Mohammad: I don't think we need the time to bounded by the cert length since the cert length
+              is bounded by input length.*)
+    "\<And>s. \<exists>t s'. (c, s) \<Rightarrow>\<^bsup> t \<^esup> s' \<and>
+                   t \<le> poly_of pt (bit_length (s ''input''))"
+  assumes verifier_terminates: 
+          (*"\<And>x z. \<forall>s. s ''input'' = x \<and> s ''certificate'' = z \<longrightarrow>
+                         (\<exists>t s'. (c, s) \<Rightarrow>\<^bsup> t \<^esup> s' \<and> s' ''input'' = in_lang x)"*)
+          (*Mohammad: The TM needs no access to the certificate since it is non-deterministic, i.e. it can
+            assume it is guessed.*)
+          (*Mohammad: The computation output should depend on the state, otherwise the theorem
+                      statement does not hold*)
+          (*Mohammad: We need to specify what it means for c to be a verifier for the certificates*)
+          "\<And>x s. \<lbrakk>in_lang x = 0 ; s ''input'' = x\<rbrakk> \<Longrightarrow>
+                    (\<exists>z t s'. bit_length z \<le> poly_of p_cer (bit_length x) \<and>
+                              (c, s(''certificate'' := z)) \<Rightarrow>\<^bsup> t \<^esup> s' \<and>
+                              s' ''input'' = in_lang x)"
+          "\<And>x s s' t. \<lbrakk>in_lang x \<noteq> 0; s ''input'' = x; (c, s) \<Rightarrow>\<^bsup> t \<^esup> s'\<rbrakk> \<Longrightarrow>
+                         s' ''input'' = in_lang x"
+  assumes verifier_has_registers:
+    "''input'' \<in> set (IMP_Minus_Max_Constant.all_variables c)"
+  shows "\<exists>t_red s_red.
+         poly t_red 
+       \<and> poly s_red
+       \<and> (\<forall>x. \<exists>f.  bit_length (encode_sat f) \<le> s_red ( bit_length x ) \<and> imp_to_sat_list c pt p_cer x = f
+                   \<and> (Sema.sat {f}  \<longleftrightarrow> in_lang x = 0))"
+  using main_lemma_hol poly_poly_of assms  by (auto simp add: sublist_imp_to_sat) 
+
+ definition imp_to_sat_nat :: "nat \<Rightarrow> nat \<Rightarrow> nat \<Rightarrow> nat \<Rightarrow> nat" where
+    "imp_to_sat_nat c pt p_cer x =
+      (let I = (prod_encode (vname_encode ''input'', x)) ## 0; 
+          G = (prod_encode (vname_encode ''input'', 0)) ## 0;
+          guess_range = x + 1 + 2 * 2 ^ (poly_of_nat p_cer (bit_length x));
+          max_bits = max_input_bits_nat c I guess_range
+      in
+        encode_problem_with_operator_interference_exclusion_nat 
+        (sas_plus_problem_to_strips_problem_nat (prob_with_noop_nat (IMP_Minus_to_SAS_Plus_nat c I guess_range G (t'_nat pt p_cer x))))
+           (100 * (max_bits + (t'_nat pt p_cer x) + 1) * ((t'_nat pt p_cer x) - 1) +
+             (max_bits + (t'_nat pt p_cer x) + 2) * (num_variables_nat c + 2) + 52))"
+lemma unfold_map_signleton:"[f x] = map f [x]"
+  apply auto
+  done
+
+lemma subnat_imp_to_sat:
+"imp_to_sat_nat (com_encode c) (prod_encode pt) (prod_encode p_cer) x =
+sat_formula_encode (imp_to_sat_list c pt p_cer x)  "
+  apply (auto simp only: imp_to_sat_nat_def Let_def
+    cons0 sub_cons  unfold_map_signleton[of impm_assignment_encode] 
+sub_poly_of subnat_max_input_bits subnat_t' sub_num_variables subnat_IMP_Minus_to_SAS_Plus
+subnat_prob_with_noop subnat_encode_problem_with_operator_interference_exclusion
+simp flip: impm_assignment_encode.simps  impm_assignment_list_encode_def
+)
+proof -
+  let ?P = "IMP_Minus_to_SAS_Plus_list c [(''input'', x)]
+              (x + 1 + 2 * 2 ^ poly_of p_cer (Bit_Length.bit_length x)) [(''input'', 0)]
+              (t'_pair pt p_cer x)"
+  let ?P'= "IMP_Minus_to_SAS_Plus c (map_of [(''input'', x)])
+              (x + 1 + 2 * 2 ^ poly_of p_cer (Bit_Length.bit_length x)) (map_of [(''input'', 0)])
+              (t'_pair pt p_cer x)"
+  have "list_problem_to_problem ?P = ?P'" using sublist_IMP_Minus_to_SAS_Plus by blast
+  hence "is_valid_problem_sas_plus (list_problem_to_problem ?P)" using valid_problem by presburger
+  hence "is_valid_problem_sas_plus (prob_with_noop (list_problem_to_problem ?P))" using noops_valid
+    by fast
+  hence "is_valid_problem_sas_plus (list_problem_to_problem (prob_with_noop_list ?P))"
+    using sublist_prob_with_noop by metis
+  thus " encode_problem_with_operator_interference_exclusion_nat
+     (\<phi> list_problem_plus_encode
+          (prob_with_noop_list
+            (IMP_Minus_to_SAS_Plus_list c [(''input'', x)]
+              (x + 1 + 2 * 2 ^ poly_of p_cer (Bit_Length.bit_length x)) [(''input'', 0)]
+              (t'_pair pt p_cer x))) )
+     (100 *
+      (max_input_bits_list c [(''input'', x)] (x + 1 + 2 * 2 ^ poly_of p_cer (Bit_Length.bit_length x)) +
+       t'_pair pt p_cer x +
+       1) *
+      (t'_pair pt p_cer x - 1) +
+      (max_input_bits_list c [(''input'', x)] (x + 1 + 2 * 2 ^ poly_of p_cer (Bit_Length.bit_length x)) +
+       t'_pair pt p_cer x +
+       2) *
+      (num_variables c + 2) +
+      52) =
+    sat_formula_encode (imp_to_sat_list c pt p_cer x)"
+    apply (auto simp only: subnat_sas_plus_problem_to_strips_problem Let_def
+          subnat_encode_problem_with_operator_interference_exclusion imp_to_sat_list_def )
+    done
+       
+qed 
+
+lemma inj_formula : "inj sat_formula_encode" 
+  apply (auto simp add: inj_def)
+  using sat_formula_id by metis
+
+lemma inj_formula_simp : "(sat_formula_encode x = sat_formula_encode y) = (x=y)"
+  using inj_formula by (auto simp add:inj_def)
+lemma main_lemma_hol_nat:
+  fixes c pt p_cer in_lang
+  assumes verifier_tbounded:
+    "\<And>s. \<exists>t s'. (c, s) \<Rightarrow>\<^bsup> t \<^esup> s' \<and>
+                   t \<le> poly_of pt (bit_length (s ''input''))"
+  assumes verifier_terminates: 
+          "\<And>x s. \<lbrakk>in_lang x = 0 ; s ''input'' = x\<rbrakk> \<Longrightarrow>
+                    (\<exists>z t s'. bit_length z \<le> poly_of p_cer (bit_length x) \<and>
+                              (c, s(''certificate'' := z)) \<Rightarrow>\<^bsup> t \<^esup> s' \<and>
+                              s' ''input'' = in_lang x)"
+          "\<And>x s s' t. \<lbrakk>in_lang x \<noteq> 0; s ''input'' = x; (c, s) \<Rightarrow>\<^bsup> t \<^esup> s'\<rbrakk> \<Longrightarrow>
+                         s' ''input'' = in_lang x"
+  assumes verifier_has_registers:
+    "''input'' \<in> set (IMP_Minus_Max_Constant.all_variables c)"
+  shows "\<exists>t_red s_red.
+         poly t_red 
+       \<and> poly s_red
+       \<and> (\<forall>x. \<exists>f.  bit_length (encode_sat f) \<le> s_red ( bit_length x ) \<and> imp_to_sat_nat (com_encode c) (prod_encode pt) (prod_encode p_cer) x = sat_formula_encode f
+                   \<and> (Sema.sat {f}  \<longleftrightarrow> in_lang x = 0))"
+  using assms main_lemma_hol_list by (auto simp add:subnat_imp_to_sat inj_formula_simp)
+
 
 end
